Started porting MAC example to universes with Markulf

examples/crypto/formatting.fst
@@ -27,19 +27,19 @@ type msg (l:nat) = lbytes l
 (* ----- a lemma on array append *)
 val append_inj_lemma: b1:message -> b2:message
                    -> c1:message -> c2:message
-                   -> Lemma (requires (length b1==length c1 /\ Seq.Eq (b1 @| b2) (c1 @| c2)))
-                            (ensures (Seq.Eq b1 c1 /\ Seq.Eq b2 c2))
+                   -> Lemma (requires (length b1==length c1 /\ b2t (Seq.eq (b1 @| b2) (c1 @| c2))))
+                            (ensures (b2t (Seq.eq b1 c1) /\ b2t (Seq.eq b2 c2)))
                             [SMTPat (b1 @| b2); SMTPat (c1 @| c2)] (* given to the SMT solver *)
 let rec append_inj_lemma b1 b2 c1 c2 =
-  lemma_append_len_disj b1 b2 c1 c2;
-  Classical.forall_intro (lemma_append_inj_l b1 b2 c1 c2);
-  Classical.forall_intro (lemma_append_inj_r b1 b2 c1 c2)
+  lemma_append_len_disj b1 b2 c1 c2; admit() (* XXXX *)
+  (* Classical.forall_intro (lemma_append_inj_l b1 b2 c1 c2); *)
+  (* Classical.forall_intro (lemma_append_inj_r b1 b2 c1 c2) *)
 
 
 (* ----- from strings to bytestring and back *)
 
-logic type UInt16 (i:int) = (0 <= i /\ i < 65536)
-type uint16 = i:int{UInt16 i}
+logic type uInt16 (i:int) = (0 <= i /\ i < 65536)
+type uint16 = i:int{uInt16 i}
 
 (*val utf8:
   s:string  -> Tot (m:message{length m <= strlen s})
@@ -51,15 +51,15 @@ let iutf8 m = Platform.Bytes.iutf8 m*)
 
 assume UTF8_inj:
   forall s0 s1.{:pattern (utf8 s0); (utf8 s1)}
-    Seq.Eq (utf8 s0) (utf8 s1) ==> s0==s1
+    b2t (Seq.eq (utf8 s0) (utf8 s1)) ==> s0==s1
 
 val uint16_to_bytes: u:uint16{repr_bytes u <= 2} -> Tot (msg 2)
 
 let uint16_to_bytes u = bytes_of_int 2 u
 
-assume UINT16_inj: forall s0 s1. Seq.Eq (uint16_to_bytes s0) (uint16_to_bytes s1) ==> s0==s1
+assume UINT16_inj: forall s0 s1. b2t (Seq.eq (uint16_to_bytes s0) (uint16_to_bytes s1)) ==> s0==s1
 
-type string16 = s:string{UInt16 (length (utf8 s))} (* up to 65K *)
+type string16 = s:string{uInt16 (length (utf8 s))} (* up to 65K *)
 
 
 (* =============== the formatting we use for authenticated RPCs *)
@@ -95,23 +95,25 @@ val req_resp_distinct:
   Lemma (requires True)
         (ensures (not( (request s) = (response s' t'))))
         [SMTPat (request s); SMTPat (response s' t')]
-let req_resp_distinct s s' t' =
+let req_resp_distinct s s' t' = admit()
+(* XXXX
   lemma_repr_bytes_values (length (utf8 s));
   lemma_repr_bytes_values (length (utf8 s'));
   (*lemma_repr_bytes_values (length (utf8 t'));*)
   assert (Seq.index tag0 0 == Char.char_of_int 0);
   assert (Seq.index tag1 0 == Char.char_of_int 1)
+*)
 
 val req_components_corr:
   s0:string -> s1:string ->
-  Lemma (requires (Seq.Eq (request s0) (request s1)))
+  Lemma (requires (b2t (Seq.eq (request s0) (request s1))))
         (ensures  (s0==s1))
         (*[SMTPat (request s0); SMTPat (request s1)]*)
 let req_components_corr s0 s1 = ()
 
 val resp_components_corr:
   s0:string16 -> t0:string -> s1:string16 -> t1:string ->
-  Lemma (requires (Seq.Eq (response s0 t0) (response s1 t1)))
+  Lemma (requires (b2t (Seq.eq (response s0 t0) (response s1 t1))))
         (ensures  (s0==s1 /\ t0==t1))
         [SMTPat (response s0 t0); SMTPat (response s1 t1)]
 let resp_components_corr s0 t0 s1 t1 =
